\documentclass[12pt]{article}
\usepackage{amsmath}
\begin{document}
\begin{title}
    \centering
    {\LARGE\bfseries Exercise 2.3.1}
\end{title}\\

\vspace{10mm} %10mm vertical space
Show the following formulas by induction on n starting at n = 1.

\vspace{5mm} %5mm vertical space

d) $\sum_{i=1}^{n}\frac{1}{i(i + 1)} = \frac{n}{(n + 1)}$\par

\vspace{5mm} %5mm vertical space

Basis case: LHS when n = 1 yields 1/2.\par

\vspace{5mm} %5mm vertical space

RHS when n = 1 is 1/2\par

LHS = RHS therefore s(n) is true when n is 1.\par

Inductive step: Assume that n $\geq$ 1 and that s(n) is true as proved above.\par I must prove that s(n + 1) is true which is:\par

\vspace{5mm} %5mm vertical space

$\sum_{i=1}^{n + 1}\frac{1}{i(i + 1)} = \frac{n + 1}{(n + 2)}$   \hfil\hfil\hfil (2)\par

\vspace{5mm} %5mm vertical space

Replacing the LHS of the above equation with the following:\par

\vspace{5mm} %5mm vertical space

$\sum_{i=1}^{n + 1}\frac{1}{i(i + 1)} = (\sum_{i=1}^{n}\frac{1}{i(i + 1)}) + \frac{1}{(n + 1)(n + 2)}$\par

\vspace{5mm} %5mm vertical space

which can be rewritten as:\par

\vspace{5mm} %5mm vertical space

$\sum_{i=1}^{n + 1}\frac{1}{i(i + 1)} = \frac{n}{(n + 1)} + \frac{1}{(n + 1)(n + 2)}$\par

\vspace{5mm} %5mm vertical space

\hfil $=  \frac{n(n + 2) + 1}{(n + 1)(n + 2)}$\par

\vspace{5mm} %5mm vertical space

\hfil $=  \frac{n^2 + 2n + 1}{(n + 1)(n + 2)}$\par

\vspace{5mm} %5mm vertical space

\hfil $=  \frac{(n + 1)^2}{(n + 1)(n + 2)}$\par

\vspace{5mm} %5mm vertical space

\hfil $=  \frac{(n + 1)}{(n + 2)}$\par

\vspace{5mm} %5mm vertical space

The final equation the right is equal to (2) proving that s(n + 1) is also\par true.
Therefore s(n) holds for all n $\geq$ 1
\end{document}